theories/BWT/Sorting/Key.v
@@ -1,9 +1,11 @@
 Require Import Coq.Lists.List.
+Require Import Coq.omega.Omega.
 
 Require Import BWT.Sorting.InsertionSort.
 Require Import BWT.Sorting.Lexicographic.
 Require Import BWT.Sorting.Ord.
 Require Import BWT.Sorting.Sorted.
+Require Import BWT.Lib.List.
 
 Section KeyOrd.
   Context {A K : Type} `{O: Ord K}.
@@ -16,31 +18,47 @@ Section KeyOrd.
       intros; eauto using le_trans, le_total, le_dec.
   Defined.
 
+  Local Arguments le {_} _.
+  Local Arguments lt {_} _.
+  Local Arguments eqv {_} _.
+  Local Arguments le_dec {_} _.
+
   Remark key_le : forall x y,
-      @le A keyOrd x y = @le K O (key x) (key y).
+      le keyOrd x y = le O (key x) (key y).
+  Proof. reflexivity. Qed.
+
+  Remark key_lt : forall x y,
+      lt keyOrd x y = lt O (key x) (key y).
+  Proof. reflexivity. Qed.
+
+  Remark key_eqv : forall x y,
+      eqv keyOrd x y = eqv O (key x) (key y).
   Proof. reflexivity. Qed.
 
   Remark key_le_dec : forall x y,
-      @le_dec A keyOrd x y = @le_dec K O (key x) (key y).
+      le_dec keyOrd x y = le_dec O (key x) (key y).
   Proof. reflexivity. Qed.
 
   Section Inv.
     Variable f : A -> A.
     Hypothesis HF : forall x, key (f x) = key x.
 
+    Local Arguments insert {_} _.
+    Local Arguments sort {_} _.
+
     Lemma key_insert_inv : forall x l,
-       @insert A keyOrd (f x) (map f l) = map f (@insert A keyOrd x l).
+       insert keyOrd (f x) (map f l) = map f (insert keyOrd x l).
     Proof.
       induction l; [reflexivity|].
       simpl. rewrite !HF.
-      destruct (le_dec (key x) (key a)).
+      destruct (le_dec _ (key x) (key a)).
       - reflexivity.
       - simpl; f_equal.
         apply IHl.
     Qed.
 
     Theorem key_sort_inv : forall l,
-        @sort A keyOrd (map f l) = map f (@sort A keyOrd l).
+        sort keyOrd (map f l) = map f (sort keyOrd l).
     Proof.
       induction l; [reflexivity|].
       simpl. rewrite <- key_insert_inv, IHl.
@@ -48,6 +66,148 @@ Section KeyOrd.
     Qed.
   End Inv.
 End KeyOrd.
+
+Section Firstn.
+  Context {A : Type} {O: Ord A}.
+
+  Local Arguments le {_} _.
+  Local Arguments lt {_} _.
+  Local Arguments eqv {_} _.
+  Local Arguments le_dec {_} _.
+
+  Theorem key_le_firstn_O : forall x y,
+      le (keyOrd (firstn 0)) x y.
+  Proof.
+    intros. rewrite key_le.
+    apply lex_le_nil.
+  Qed.
+
+  Theorem key_le_firstn_1 : forall hx hy tx ty,
+      le (keyOrd (firstn 1)) (hx :: tx) (hy :: ty) ->
+      le _ hx hy.
+  Proof.
+    intros. rewrite key_le in H. cbn in H.
+    inversion H; subst.
+    - apply lt_le; auto.
+    - unfold eqv in H3; intuition.
+  Qed.
+
+  Theorem key_lt_firstn_1 : forall hx hy tx ty,
+      lt (keyOrd (firstn 1)) (hx :: tx) (hy :: ty) ->
+      lt _ hx hy.
+  Proof.
+    intros. rewrite key_lt in H; cbn in H.
+    intro c.
+    apply H.
+    apply lt_spec in c.
+    destruct c.
+    - apply lex_le_cons_lt. auto.
+    - apply lex_le_cons_eq. auto. constructor.
+  Qed.
+
+  Theorem key_eqv_firstn_1 : forall hx hy tx ty,
+      eqv (keyOrd (firstn 1)) (hx :: tx) (hy :: ty) ->
+      eqv _ hx hy.
+  Proof.
+    intros. rewrite key_eqv in H.
+    cbn in H. destruct H.
+    apply key_le_firstn_1 with (tx := nil) (ty := nil) in H.
+    apply key_le_firstn_1 with (tx := nil) (ty := nil) in H0.
+    unfold eqv. intuition.
+  Qed.
+
+  Theorem key_le_firstn_gt : forall j x y,
+      le (keyOrd (firstn (S j))) x y ->
+      le (keyOrd (firstn j)) x y.
+  Proof.
+    intros.
+    rewrite key_le in *.
+    apply lt_spec in H.
+    destruct H.
+    apply lex_lt_destr in H.
+    destruct H as [hx [tx [hy [ty [Hx [Hy [Hlt Heq]]]]]]].
+    remember (length hx) as n.
+    assert (Heqn' : n = length hy). {
+      apply lex_eqv_iff in Heq.
+      subst n. eapply Forall2_length; eauto.
+    }
+    destruct (Nat.le_gt_cases (S j) n).
+    + assert (HT: tx = nil /\ ty = nil). {
+        apply f_equal with (f := @length A) in Hx; apply f_equal with (f := @length A) in Hy.
+        rewrite app_length in *.
+        rewrite <- Heqn in Hx. rewrite <- Heqn' in Hy.
+        pose proof (firstn_le_length (S j) x).
+        pose proof (firstn_le_length (S j) y).
+        split; apply length_zero_iff_nil; omega.
+      }
+      destruct HT; subst tx ty.
+      rewrite app_nil_r in *.
+      apply f_equal with (f := firstn j) in Hx; apply f_equal with (f := firstn j) in Hy.
+      rewrite firstn_firstn in *.
+      replace (Nat.min j (S j)) with j in * by (symmetry; apply Nat.min_l; omega).
+      rewrite Hx, Hy.
+      apply lex_eqv_firstn. symmetry. auto.
+    +
+      pose proof (firstn_le_length (S j) x).
+      rewrite firstn_all2 in Hx.
+
+
+
+    destruct x as [|a x]; [rewrite firstn_nil; constructor|].
+    destruct y as [|b y]; [symmetry in Hy; apply app_eq_nil in Hy; destruct Hy; subst; apply lex_lt_iff in Hlt; inversion Hlt|].
+    cbn in Hx; cbn in Hy.
+    destruct hx as [|hxhd hxtl].
+    replace hy with (@nil A) in * by (apply lex_eqv_iff in Heq; inversion Heq; auto).
+
+
+
+    cbn in Hx.
+    rewrite key_le.
+    destruct (Nat.lt_ge_cases (S j))
+    Search "<".
+    destruct ()
+
+    pose proof (lex_)
+    rewrite key_le in H.
+    destruct (Nat.le_gt_cases (length x) (S j)).
+    - rewrite firstn_all2 in H by omega.
+
+      r
+        ewrite firstn_length_le in H.
+
+  Theorem key_le_firstn_gt : forall k j x y,
+      j < k ->
+      le (keyOrd (firstn k)) x y ->
+      le (keyOrd (firstn j)) x y.
+  Proof.
+    induction k; intros j x y HJK HLeK.
+    - assert (j = 0) by omega.
+      subst j. apply key_le_firstn_O.
+    - apply le_lt_or_eq in HJK.
+      destruct HJK.
+      apply IHk. omega.
+      admit.
+      inversion H; subst.
+
+
+  Theorem key_firstn_S : forall n x y,
+      le (keyOrd (firstn 1)) x y ->
+      le (keyOrd (firstn n)) (tl x) (tl y) ->
+      le (keyOrd (firstn (S n))) x y.
+  Proof.
+    induction n; intros x y L1 Ln; [auto|].
+    remember (S n) as n'.
+    destruct x as [|hx tx]; [apply lex_le_nil|].
+    destruct y as [|hy ty]; [apply lex_le_not_nil_r in L1; contradiction|].
+    rewrite key_le; cbn.
+    apply lt_spec in L1; destruct L1 as [HLt | HEq].
+    - apply lex_le_cons_lt.
+      apply key_lt_firstn_1 in HLt. auto.
+    - apply lex_le_cons_eq.
+      apply key_eqv_firstn_1 in HEq. auto.
+      apply IHn. cbn in Ln. app
+
+End Firstn.
 
 Section HdSort.
   Context {A : Type} `{O: Ord A}.
@@ -62,16 +222,15 @@ Section Prefix.
 
   Local Arguments Sorted {_} _ _.
 
-  Definition prefixSorted (n : nat) : list (list A) -> Prop
+  Definition PrefixSorted (n : nat) : list (list A) -> Prop
     := Sorted (keyOrd (firstn n)).
 
-  Theorem prefixSorted_zero : forall l,
-      prefixSorted 0 l.
+  Theorem PrefixSorted_zero : forall l,
+      PrefixSorted 0 l.
   Proof.
-    intros l. unfold prefixSorted.
+    intros l. unfold PrefixSorted.
     induction l; [apply Sorted_nil|].
     apply Sorted_cons.
-    intros. rewrite key_le.
-    apply lex_le_nil. apply IHl.
+    intros. apply key_firstn_O. apply IHl.
   Qed.
 End Prefix.
