theories/BWT/Sorting/Lexicographic.v
@@ -17,8 +17,8 @@ Section LexLe.
 
   Inductive lex_le : list A -> list A -> Prop :=
   | lex_le_nil : forall ys, lex_le [] ys
-  | le_cons_lt : forall x y xs ys, lt x y -> lex_le (x :: xs) (y :: ys)
-  | le_cons_eq : forall x y xs ys, eqv x y -> lex_le xs ys ->
+  | lex_le_cons_lt : forall x y xs ys, lt x y -> lex_le (x :: xs) (y :: ys)
+  | lex_le_cons_eq : forall x y xs ys, eqv x y -> lex_le xs ys ->
                               lex_le (x :: xs) (y :: ys).
 
   Theorem lex_le_trans : forall x y z, lex_le x y -> lex_le y z -> lex_le x z.
@@ -27,10 +27,10 @@ Section LexLe.
     induction LXY as [|x y xs ys HLT|x y xs ys HE HLex IH]; intros z LYZ;
       [constructor|inversion LYZ; subst; clear LYZ..];
       rename y0 into z; rename ys0 into zs.
-    - apply le_cons_lt. eapply lt_trans; eauto.
-    - apply le_cons_lt. rewrite <- H1. auto.
-    - apply le_cons_lt. rewrite HE. auto.
-    - apply le_cons_eq.
+    - apply lex_le_cons_lt. eapply lt_trans; eauto.
+    - apply lex_le_cons_lt. rewrite <- H1. auto.
+    - apply lex_le_cons_lt. rewrite HE. auto.
+    - apply lex_le_cons_eq.
       eapply eqv_trans; eauto.
       apply IH; auto.
   Defined.
@@ -39,8 +39,8 @@ Section LexLe.
   Proof.
     induction x as [|x xs]; [left; constructor|].
     intros [|y ys]; [right; constructor|].
-    destruct (lt_eq_dec x y) as [[LXY|E]|LYX]; eauto using le_cons_lt.
-    edestruct IHxs; eauto using le_cons_eq, eqv_sym.
+    destruct (lt_eq_dec x y) as [[LXY|E]|LYX]; eauto using lex_le_cons_lt.
+    edestruct IHxs; eauto using lex_le_cons_eq, eqv_sym.
   Defined.
 
   Program Fixpoint lex_le_dec xs ys : { lex_le xs ys } + { ~ lex_le xs ys } :=
@@ -60,18 +60,68 @@ Section LexLe.
     end.
   Next Obligation. constructor. Defined.
   Next Obligation. intro c; inversion c. Defined.
-  Next Obligation. apply le_cons_lt. auto. Defined.
+  Next Obligation. apply lex_le_cons_lt. auto. Defined.
   Next Obligation.
     intro c. inversion c; subst; clear c.
     - eapply lt_excl; split; eauto.
     - eapply lt_not_eq; eauto using eqv_sym.
   Defined.
-  Next Obligation. apply le_cons_eq; auto. Defined.
+  Next Obligation. apply lex_le_cons_eq; auto. Defined.
   Next Obligation.
     intro c. inversion c; subst; clear c.
     - eapply lt_not_eq; eauto.
     - contradiction.
   Defined.
+
+  Theorem lex_le_not_nil_r : forall (a : A) x,
+      ~ lex_le (a :: x) [].
+  Proof. intros. intro c. inversion c. Qed.
+
+  Theorem lex_le_trunc_r : forall x y,
+      lex_le x y ->
+      lex_le x (firstn (length x) y).
+  Proof.
+    induction x; intros y HLE; [apply lex_le_nil|].
+    inversion HLE; subst.
+    - cbn. apply lex_le_cons_lt. auto.
+    - cbn. apply lex_le_cons_eq. auto.
+      apply IHx. auto.
+  Qed.
+
+  Inductive lex_lt : list A -> list A -> Prop :=
+  | lex_lt_nil : forall hy ty, lex_lt [] (hy :: ty)
+  | lex_lt_cons_lt : forall x y xs ys, lt x y -> lex_lt (x :: xs) (y :: ys)
+  | lex_lt_cons_eq : forall x y xs ys, eqv x y -> lex_lt xs ys ->
+                              lex_lt (x :: xs) (y :: ys).
+
+  Theorem lex_lt_iff : forall x y,
+      lex_lt x y <-> ~ (lex_le y x).
+  Proof.
+    induction x; intro y.
+    - split.
+      + intro. inversion H.
+        apply lex_le_not_nil_r.
+      + intro. destruct y.
+        exfalso; apply H; constructor.
+        constructor.
+    - split.
+      + intro. inversion H; subst; clear H.
+        * intro c.
+          inversion c; subst; clear c.
+          apply (lt_excl a y0); split; auto.
+          apply (lt_not_eq a y0); auto. symmetry. auto.
+        * intro c. inversion c; subst; clear c.
+          apply (lt_not_eq y0 a); auto. symmetry; auto.
+          apply IHx in H4. contradiction.
+      + intro. destruct y. exfalso. apply H. constructor.
+        destruct (le_dec a0 a).
+        apply lt_spec in l. destruct l.
+        exfalso. apply H. apply lex_le_cons_lt. auto.
+        apply lex_lt_cons_eq. symmetry. auto.
+        apply IHx.
+        intro c. apply H. apply lex_le_cons_eq; auto.
+        apply lex_lt_cons_lt. auto.
+  Qed.
 End LexLe.
 
 Instance Ord_list_lex {A} `{Ord A} : Ord (list A) :=
@@ -103,3 +153,102 @@ Section LexSort.
     apply Permutation_sym. apply lexsort_perm.
   Qed.
 End LexSort.
+
+Theorem lex_lt_inv {A : Type} {O : Ord A} : forall hx tx hy ty,
+    lt (hx :: tx) (hy :: ty) ->
+    (eqv hx hy /\ lt tx ty) \/ lt hx hy.
+Proof.
+  intros. apply lex_lt_iff in H.
+  remember (hx :: tx) as x.
+  remember (hy :: ty) as y.
+  revert hx tx hy ty Heqx Heqy.
+  induction H; [discriminate|intros hx tx hy ty Heqx Heqy; inversion Heqx; inversion Heqy; subst; clear Heqx Heqy..].
+  - right; auto.
+  - destruct tx. inversion H0; subst; clear H0.
+    left. split; auto.
+    apply lex_lt_iff. constructor.
+    destruct ty. inversion H0.
+    destruct (IHlex_lt a tx a0 ty) as [[]|]; auto.
+    + left; split; auto.
+      apply lex_lt_iff.
+      apply lex_lt_iff in H2.
+      apply lex_lt_cons_eq; auto.
+    + left; split; auto.
+      apply lex_lt_iff.
+      apply lex_lt_cons_lt.
+      auto.
+Qed.
+
+Theorem lex_lt_destr {A : Type} {O : Ord A} : forall x y : list A,
+    lt x y ->
+    exists hx tx hy ty,
+      x = hx ++ tx /\
+      y = hy ++ ty /\
+      lt tx ty /\
+      eqv hx hy.
+Proof.
+  intros x y HLT. apply lex_lt_iff in HLT.
+  induction HLT.
+  - exists [], [], [], (hy::ty).
+    repeat split; [apply lex_lt_iff|..]; constructor.
+  - exists [], (x::xs), [], (y::ys).
+    repeat split; [apply lex_lt_iff|..]; constructor; auto.
+  - destruct IHHLT as [hx [tx [hy [ty [Hx [Hy [Hlt Heqv]]]]]]].
+    exists (x::hx), tx, (y::hy), ty.
+    rewrite Hx, Hy.
+    repeat split; [|apply lex_le_cons_eq..];
+      auto using eqv_rel_Symmetric; destruct Heqv; auto.
+Qed.
+
+Theorem lex_eqv_iff {A} {O : Ord A} : forall x y,
+    Forall2 eqv x y <-> eqv x y.
+Proof.
+  induction x as [|a x IH]; intros y.
+  - split.
+   + intro H. inversion H; subst.
+     split; constructor.
+   + intros [LXY LYX].
+     inversion LYX; subst.
+     constructor.
+  - split.
+    + intro H. inversion H; subst; clear H.
+      apply IH in H4. destruct H4.
+      split; apply lex_le_cons_eq; auto using eqv_rel_Symmetric.
+    + intros [LXY LYX].
+      inversion LXY; inversion LYX; subst.
+      * discriminate.
+      * inversion H4; subst.
+        exfalso; apply (lt_excl a y0); auto.
+      * inversion H5; subst.
+        symmetry in H6. apply lt_not_eq in H6. contradiction.
+        auto.
+      * discriminate.
+      * inversion H5; subst.
+        symmetry in H1; apply lt_not_eq in H1. contradiction. auto.
+      * inversion H6; subst.
+        assert (eqv x ys) by (split; auto).
+        constructor; auto. apply IH. auto.
+Qed.
+
+Theorem lex_eqv_prepend {A} {O : Ord A} : forall hx tx hy ty,
+    eqv hx hy -> le tx ty -> le (hx ++ tx) (hy ++ ty).
+Proof.
+  intros hx tx hy ty HE.
+  apply lex_eqv_iff in HE.
+  induction HE; intro HL.
+  - cbn. auto.
+  - cbn. apply lex_le_cons_eq; auto.
+    apply IHHE. auto.
+Qed.
+
+Theorem lex_eqv_firstn {A} {O : Ord A} : forall x y j,
+    eqv x y ->
+    eqv (firstn j x) (firstn j y).
+Proof.
+  intros x y j HE; revert j.
+  apply lex_eqv_iff in HE.
+  induction HE; intros j.
+  - rewrite firstn_nil. split; constructor.
+  - apply lex_eqv_iff. destruct j; cbn; [constructor|].
+    constructor; auto. apply lex_eqv_iff. auto.
+Qed.
