theories/BWT/Sorting/RadixSort.v
@@ -10,6 +10,8 @@ Require Import BWT.Rotation.Rotation.
 Require Import BWT.Lib.Repeat.
 Require Import BWT.Sorting.Key.
 Require Import BWT.Lib.List.
+Require Import BWT.Columns.
+Require Import BWT.Sorting.Lexicographic.
 
 Section RadixSort.
   Context {A : Type} {O : Ord A}.
@@ -44,6 +46,55 @@ Section RadixSort.
     cbn; intros a HN.
     rewrite <- HN. symmetry. apply rrot_rep_id.
   Qed.
+
+  Local Arguments eqv {_} _.
+  Local Arguments le {_} _.
+  Local Arguments lt {_} _.
+  Local Arguments StablePerm {_} _ {_}.
+  Local Arguments tl {_}.
+
+  Theorem hdsort_sorted_S : forall n colmat colmat',
+      StablePerm (eqv (keyOrd (firstn 1))) colmat colmat' ->
+      PrefixSorted n (map tl colmat) ->
+      PrefixSorted 1 colmat' ->
+      PrefixSorted (S n) colmat'.
+  Proof.
+    intros n colmat colmat' HSP.
+    induction HSP as [| x colmat colmat' | |]; intros HPSmat HPScolmat'.
+    - apply Sorted_nil.
+    - apply Sorted_cons.
+      intros b HB.
+      inversion HPScolmat'; subst; clear HPScolmat'.
+      specialize (H1 b HB).
+      apply lt_spec in H1.
+      destruct H1.
+      + rewrite key_le.
+        unfold le, Ord_list_lex.
+        apply lex_le_cons_lt.
+
+
+
+
+
+    assert (HSP : @StablePerm _ (@eqv _ (keyOrd (firstn 1))) _ (prepend_col col mat) (hdsort (prepend_col col mat)))
+           by apply sort_stable.
+    remember (prepend_col col mat) as bigmat.
+    remember (hdsort (prepend_col col mat)) as bigmat'.
+    revert Heqbigmat Heqbigmat'.
+    induction HSP as [|x mattl mat' | x y mattl | mattl mat' mat''].
+    - intros. apply Sorted_nil.
+    - intros Hbigmat Hbigmat' n HPS.
+      unfold hdsort.
+      rewrite <- HL'.
+      apply Sorted_cons.
+      pose proof (@sort_sorted _ (keyOrd (firstn 1)) (x :: l)).
+      inversion H. cbn in HL'.
+      rewrite <- HL' in H1.
+      inversion H1.
+      cbn in HL'.
+      rewrite <- HL' in H0.
+      inversion H0; subst.
+      apply H1.
 
   Theorem radixsort_sorted : forall n l,
       Forall (fun x => length x = n) l ->
